definition of path and starting to create bfs function

LeanGraph.lean
@@ -11,17 +11,31 @@ structure edge where
 
 structure graph where
   edges : List edge
-  deriving Repr
+  deriving Repr, DecidableEq
 
-def node.eqv (n1: node) (n2: node) : Bool := n1.name = n2.name
+structure path where
+  nodes : List node
+  deriving Repr, DecidableEq
 
 def edge.rev (e : edge) : edge where
   a := e.b
   b := e.a
 
+def node.eqv (n1: node) (n2: node) : Bool := n1.name = n2.name
+
 def edge.eqv (e1: edge) (e2: edge) : Bool := e1 = e2 ∨ e1.rev = e2
 
 def edge.hasNode (e: edge) (n: node) : Bool := e.a.eqv n ∨ e.b.eqv n
+
+def edge.listNodes (e: edge) : List node := [e.a, e.b]
+
+theorem edgeHasAlwaysTwoNodes : ∀e : edge, (e.listNodes.length = 2) := by
+  intro e; unfold edge.listNodes; simp;
+
+def edge.otherNode (e: edge) (n: node) : node :=
+  let other := (e.listNodes.filter (fun node : node => ¬(n.eqv node)));
+  have : 0 < other.length := by sorry;
+  other[0]
 
 def graph.hasEdge (e : edge) (g : graph) : Bool :=
   match he : g.edges with
@@ -43,6 +57,46 @@ def graph.hasNode (n: node) (g: graph) : Bool :=
     h.hasNode n ∨ hasNode n {g with edges:= t}
   termination_by g.edges.length
 
+def graph.filterSameEdges (e: edge) (g: graph) : List edge := g.edges.filter (fun edge : edge => e.eqv edge)
+
+def graph.ocurrencesOfEdge (e: edge) (g: graph) : Int := (g.filterSameEdges e).length
+
+def graph.edgeIsUnique (e: edge) (g: graph) : Bool := (g.filterSameEdges e) = [e]
+
+def graph.isProper (g: graph) : Bool := g.edges.all g.edgeIsUnique
+
+def graph.incidentEdgesOnNode (n: node) (g: graph) : List edge := g.edges.filter (fun e : edge => e.hasNode n)
+
+def graph.allNeighborsOfNode (n: node) (g: graph) : List node := ((g.incidentEdgesOnNode n).map (fun e : edge => e.otherNode n)).flatten
+
+def graph.areNeighbors (n1: node) (n2: node) (g: graph) : Bool := g.edges.any (fun e : edge =>
+  have possibleEdge : edge := {a:= n1, b:= n2}; e.eqv possibleEdge
+)
+
+def path.isProper (g: graph) (p: path) : Bool :=
+  match he : p.nodes with
+  | [] => true
+  | _ :: [] => true
+  | h :: h₁ :: t =>
+    have : (h₁::t).length < p.nodes.length := by
+      rw [he]
+      simp
+  g.areNeighbors h h₁ ∧ isProper g {p with nodes:=h₁::t}
+  termination_by p.nodes.length
+
+
+
+def graph.acessibleFromNode (g: graph) (n: node) : List edge :=
+  let bfs (current: node) (unvisited: List edge) (result: List edge) : List edge :=
+    let neighbors : List node := g.allNeighborsOfNode current;
+    let currentVisitedEdges : List edge := g.incidentEdgesOnNode current;
+    let newUnvisitedEdges : List edge := unvisited.removeAll currentVisitedEdges;
+    let result := currentVisitedEdges ++ (newUnvisitedEdges.map (fun e : edge =>
+      bfs (e.otherNode current)
+    )).flatten
+
+  -- Unfinished...
+
 
 def nullName : Int := 0
 def nullNode : node := {name := nullName}
@@ -56,4 +110,9 @@ def edge_2 : edge := {a:=testNode2, b:=testNode3}
 def edge_3 : edge := {a:=testNode3, b:=testNode}
 
 def nullGraph : graph := {edges:=[]}
-def example_graph : graph := {edges:=[edge_1, edge_2]}
+def example_graph : graph := {edges:=[edge_1, edge_2, edge_3]}
+def example_path : path := {nodes:=[testNode, testNode2]}
+
+#eval example_graph.edgeIsUnique edge_1
+#eval example_path.isProper example_graph
+#eval ([edge_1] ++ [edge_2])
